%!TEX program = xelatex
\documentclass[lang=cn,12pt]{elegantpaper}
\usepackage{Onns}
\title{概率图模型}
\date{\today}

\author{刘潘}
\university{厦门大学}
\academy{信息科学与技术学院}
\majorin{计算机技术专业}
\grade{2018级研究生}
\course{机器学习}
\xmuid{23020181154229}
\titlenote{}

\begin{document}

\titleN

\section*{问题一}

\subsection*{解答}

\begin{enumerate}
	\item \begin{align}
		p(v,h) = \frac{1}{Z}exp\left\{ -E(v,h) \right\}
	\end{align}
	
	\begin{align}
		E(v,h) & = -v^TWh-a^Tv-b^Th \\
		 & = -\sum_i\sum_jh_iW_{ji}v_j - \sum_ja_jv_j - \sum_ib_ih_i
	\end{align}
	
	\begin{align*}
		E(v,h) & = -v^TWh-a^Tv-b^Th \\
		 & = -\sum_i\sum_jh_iW_{ji}v_j - \sum_ja_jv_j - \sum_ib_ih_i
	\end{align*}
	
	\begin{align*}
		Z = \sum_{v,h}exp \left\{-E(v,h) \right\}
	\end{align*}
	
	\begin{align*}
		h_{-k} = (h1,h2,\cdots,h_{k-1},h_{k+1},\cdots,h_{n_k})^T
	\end{align*}
	
	\begin{align*}
		\alpha_k(v) = b_k + \sum_jW_{jk}v_j
	\end{align*}
	
	\begin{align*}
		\beta(v,h_{-k}) = \sum_ja_jv_j + \sum_{i-1,i\neq k} b_ih_i + \sum_{i,i\neq k} \sum_jh_iW_{ji}v_j 
	\end{align*}
	
	\begin{align*}
		E(v,h) = - \beta(v,h_{-k}) - h_k \alpha_k(v)
	\end{align*}
	
	
	\begin{align*}
		p(h_i=1|v) & = p(h_i=1|h_{-i},v)  \\
		& = \frac{p(h_i=1,h_{-i},v)}{p(h_{-i},v)}  \\
		& = \frac{p(h_i=1,h_{-i},v)}{p(h_i=1,h_{-i},v) + p(h_i=0,h_{-i},v)}  \\
		& = \frac{exp\left\{ -E(h_i=1,h_{-i},v)\right\}}{exp\left\{ -E(h_i=1,h_{-i},v)\right\} + exp\left\{ -E(h_i=0,h_{-i},v)\right\}}  \\
		& = \frac{1}{exp\left\{ -E(h_i=1,h_{-i},v)  + E(h_i=0,h_{-i},v)\right\}}  \\
		& = \frac{1}{ 1+ exp\left\{ \beta(v,h_{-i}) + 0\cdot \alpha_i(v) - \beta(v,h_{-i}) - 1\cdot \alpha_i(v) \right\}}  \\
		& = \frac{1}{ 1+ exp\left\{ -\alpha_i(v) \right\}}  \\
	\end{align*}

	\item \begin{align*}
	p(v|h) = \prod_ip(v_j|h)
	\end{align*}

	\item \begin{align*}
		p(h) & = \sum_vp(v,h) \\
		& = \frac{1}{Z}\sum_v exp \left\{-E(v,h) \right\} \\
		& = \frac{1}{Z}\sum_v exp \left\{ \sum_ja_jv_j + \sum_i b_ih_i + \sum_i \sum_jh_iW_{ji}h_j  \right\} \\
		& = \frac{1}{Z}\sum_{v_1}\sum_{v_2}\cdots\sum_{v_{n_v}} exp \left\{ \sum_i b_ih_i \right\} exp \left\{ \sum_jv_j \cdot\left(a_j + \sum_ih_iW_{ji}h_j\right) \right\} \\
		& = \frac{1}{Z} exp \left\{ \sum_i b_ih_i \right\} \sum_{v_1}\sum_{v_2}\cdots\sum_{v_{n_v}}  exp \left\{ \sum_jv_j \cdot\left(a_j + \sum_ih_iW_{ji}h_j\right) \right\} \\
		& = \frac{1}{Z} exp \left\{ \sum_i b_ih_i \right\} \sum_{v_1}exp \left\{ v_1 \cdot \left(a_1 + \sum_ih_iW_{1i}h_j \right) \right\} \sum_{v_2}exp \left\{ v_2 \cdot \left(a_2 + \sum_ih_iW_{2i}h_j \right) \right\} \cdots \\ 
		& \sum_{v_{n_v}}exp \left\{ v_{n_v} \cdot \left(a_{n_v} + \sum_ih_iW_{n_vi}h_j \right) \right\}\\
		& = \frac{1}{Z} exp \left\{ \sum_i b_ih_i \right\} \prod_j\sum_{v_j}exp \left\{ v_j \cdot \left(a_j + \sum_ih_iW_{ji}h_j \right) \right\} \\ 
		& = \frac{1}{Z} \prod_i exp \left\{ b_ih_i \right\} \prod_j \left[ exp \left\{ 0 \cdot \left(a_j + \sum_ih_iW_{ji}h_j \right) \right\} + exp \left\{ 1 \cdot \left(a_j + \sum_ih_iW_{ji}h_j \right) \right\} \right]\\ 
		& = \frac{1}{Z} \prod_i exp \left\{ b_ih_i \right\} \prod_j \left[ 1 + exp \left\{ a_j + \sum_ih_iW_{ji}h_j  \right\} \right]\\ 
		\end{align*}

		\item 可以
\end{enumerate}



\section*{问题二}

\subsection*{解答}

\begin{align*} 
	arg \mathop{max}\limits_{\mathcal X} p(\mathcal X | \mathcal Y) & = arg \mathop{max}\limits_{\mathcal X} p(\mathcal X , \mathcal Y) \\
	& = \frac{1}{Z} \left[ \prod_{i=1}^D \phi(x_i,y_i) \right] \left[ \sum_{i \sim j}^D \psi(x_i,y_i) \right] \\
	& \propto \sum_{i=1}^D \beta x_iy_i + \sum_{i \sim j} \alpha x_ix_j \\
\end{align*}

\section*{问题三}

\subsection*{解答}

\begin{align*}
	\mu_{f_1 \rightarrow a}(a) & = \sum_b f_1(a,b)\mu_{b \rightarrow f_1}(b) \\ 
	\mu_{b \rightarrow f_1}(a) & = \mu_{f_2 \rightarrow b}(b) \\ 
	\mu_{f_2 \rightarrow b}(b) & = \sum_{c,d}f_2(b,c,d)\mu_{c \rightarrow f_2}(c)\mu_{d \rightarrow f_2}(d) \\ 
	\mu_{c \rightarrow f_2}(c) & = \mu_{f_3 \rightarrow c}(c) \\
	\mu_{f_3 \rightarrow c}(c) & = f_3(c) \\
	\mu_{d \rightarrow f_2}(d) & = \mu_{f_5 \rightarrow d}(d)\mu_{f_4 \rightarrow d}(d) \\
	\mu_{f_5 \rightarrow d}(d) & = f_5(d) \\
	\mu_{f_4 \rightarrow d}(d) & = \sum_ef_4(d,e)\mu_{e \rightarrow f_4}(e) \\
	\mu_{e \rightarrow f_4}(e) & = 1
\end{align*}

% \nocite{*}
% \bibliographystyle{unsrt}
% \bibliography{reference}

\end{document}